Minor changes.

ref_impl/src/verifier/fstar_files/trigger_example.fst
@@ -4,10 +4,15 @@ type list 'a : Type =
 | LNil 
 | LCons : hd : 'a -> tl : list 'a -> list 'a 
 
-val length : list 'a -> Tot int
+val length : list 'a -> Tot nat
 let rec length x = match x with
 | LNil -> 0
 | LCons _ tl -> 1 + length tl
+
+val append : list 'a -> list 'a -> list 'a
+let rec append x y = match x with
+| LNil -> y
+| LCons hd tl -> LCons hd (append tl y)
 
 val filter : ('a -> bool) -> list 'a -> list 'a
 let rec filter p x = match x with
@@ -19,40 +24,28 @@ let rec map f x = match x with
 | LNil -> LNil
 | LCons hd tl -> LCons (f hd) (map f tl)
 
-val length_is_always_positive : x : list 'a -> 
-  Lemma (requires True) (ensures length x >= 0)
-let rec length_is_always_positive x = match x with
+val length_append : x : list 'a -> y : list 'a -> Lemma (requires True) (ensures length x + length y = length (append x y)) [SMTPat (append x y)]
+let rec length_append x y = match x with
 | LNil -> ()
-| LCons _ tl -> length_is_always_positive tl
+| LCons hd tl -> length_append tl y
 
-val filtered_lists_are_smaller : p : ('a -> bool) -> x : list 'a -> 
-  Lemma (requires True) (ensures length x >= length (filter p x))
+val filter_append : p : ('a -> bool) -> x : list 'a -> y : list 'a 
+  -> Lemma (requires True) (ensures (append (filter p x) (filter p y)) == (filter p (append x y)))
+let rec filter_append p x y = match x with 
+| LNil -> ()
+| LCons hd tl ->  filter_append p tl y
+
+val filtered_lists_are_smaller : 
+p : ('a -> bool) -> x : list 'a -> Lemma (requires True) (ensures length x >= length (filter p x)) [SMTPat (filter p x)]
 let rec filtered_lists_are_smaller p x = match x with
 | LNil -> ()
 | LCons hd tl -> filtered_lists_are_smaller p tl
 
-val map_preserves_length : f : ('a -> 'b) -> x : list 'a -> 
-  Lemma (requires True) (ensures length x = length (map f x))
+val map_preserves_length : f : ('a -> 'b) -> x : list 'a 
+  -> Lemma (requires True) (ensures length x = length (map f x)) [SMTPat (map f x)]
 let rec map_preserves_length f x = match x with 
 | LNil -> ()
 | LCons hd tl -> map_preserves_length f tl
-
-// val length_is_always_positive : x : list 'a -> Lemma (requires True) (ensures length x >= 0) [SMTPat (length x)]
-// let rec length_is_always_positive x = match x with
-// | LNil -> ()
-// | LCons _ tl -> length_is_always_positive tl
-
-// val filtered_lists_are_smaller : 
-// p : ('a -> bool) -> x : list 'a -> Lemma (requires True) (ensures length x >= length (filter p x)) [SMTPat (filter p x)]
-// let rec filtered_lists_are_smaller p x = match x with
-// | LNil -> ()
-// | LCons hd tl -> filtered_lists_are_smaller p tl
-
-// val map_preserves_length : f : ('a -> 'b) -> x : list 'a -> 
-//   Lemma (requires True) (ensures length x = length (map f x)) [SMTPat (map f x)]
-// let rec map_preserves_length f x = match x with 
-// | LNil -> ()
-// | LCons hd tl -> map_preserves_length f tl
 
 val positive_fun : x : list 'a -> Tot nat
 let positive_fun x = length x
